strlen_proofs.v
@@ -54,44 +54,6 @@ Qed.
 
 
 
-(* Injections on certain data types occur frequently in proofs.  Some versions of Coq check
-   injection-heavy proofs very slowly (at Qed).  This slow-down can be avoided by sequestering
-   the most prevalent injections into lemmas, which we do here. *)
-Lemma inj_prog_stmt: forall (sz1 sz2: N) (q1 q2: stmt),
-                     Some (sz1,q1) = Some (sz2,q2) -> sz1=sz2 /\ q1=q2.
-Proof. injection 1 as. split; assumption. Qed.
-
-(* Create a case distinction between unfinished and not-unfinished program states.
-   "Unfinished" programs are those whose starting states were not provided a sufficiently
-   high recursion limit to fully evaluate one or more IL blocks.  A real CPU has no such
-   recursion limit, so we don't usually care about such states.  Proof goals therefore
-   tend to have the form "if not unfinished, then <some correctness property>". *)
-Lemma fin_dec: forall x, {x = Some Unfinished} + {x <> Some Unfinished}.
-Proof.
-  intro. destruct x; [destruct e|]; first [ left;reflexivity | right;discriminate 1].
-Qed.
-
-(* Tactic: destN n until T hyp:H
-   Keep destructing n:N until either n is a completed numeric constant (provided as an
-   equality in hypothesis H) or tactic T solves the goal.  This yields a set of subgoals
-   in which n equals the various constants admitted by T.  Typical usage:
-     destN a until (discriminate IL) hyp:ADDR.
-   where IL is an instruction lookup of the form (IL: program a = Some _). *)
-Tactic Notation "destN" constr(n) "until" tactic(T) "eqn" ":" ident(H) :=
-  let p := fresh n in
-  destruct n as [|p] eqn:H;
-  [ try solve [T]
-  | repeat first [ solve[T] | destruct p as [p|p|] ] ].
-
-(* Tactic: focus_addr H n
-   Shelve all goals except the goal in which hypothesis H has the form (H: _ = n).
-   This retrieves the subgoal for address n from a sea of arbitrarily ordered goals.
-   Use vernacular command "Unshelve" to pull back all the shelved goals afterward. *)
-Tactic Notation "focus_addr" hyp(H) constr(n) :=
-  match type of H with _ = n => idtac | _ => shelve end.
-
-
-
 (* Example #3: Architectural calling convention compliance
    Strlen does not write to callee-save registers (e.g., EBX)
    and it restores ESP on exit. *)
@@ -112,85 +74,65 @@ Proof.
   prove_noassign.
 Qed.
 
+
 (* Proving that strlen restores ESP on exit is our first example of a property that
    requires stepwise symbolic interpretation of the program to verify.  We first
    define a set of invariants, one for each program point.  In this simple case,
    all program points have the same invariant, so we return the same one for all. *)
-Definition strlen_esp_invset (esp:N) (_:addr) (_:exit) (s:store) (_:nat) :=
-  Some (s R_ESP = Ⓓ esp).
+Definition esp_invs (esp:N) (_:addr) (s:store) := Some (s R_ESP = Ⓓ esp).
 
 (* Next, we define the post-condition we wish to prove: *)
-Definition strlen_esp_postcond (esp:N) (_:addr) (_:exit) (s:store) (_:nat) :=
-  s R_ESP = Ⓓ (esp ⊕ 4).
+Definition esp_post (esp:N) (_:exit) (s:store) := s R_ESP = Ⓓ (esp ⊕ 4).
 
 (* The invariant set and post-condition are combined into a single invariant-set
-   using the x86_subroutine_inv function, which expects the subroutine's return
-   address as its third argument. *)
-Definition strlen_esp_inv (mem:addr->N) (esp:N) :=
-  x86_subroutine_inv strlen_i386 (strlen_esp_invset esp) (strlen_esp_postcond esp) (mem Ⓓ[esp]).
+   using the "invs" function. *)
+Definition strlen_esp_invset esp :=
+  invs (esp_invs esp) (esp_post esp).
 
 (* Now we pose a theorem that asserts that this invariant-set is satisfied at
-   all points where it is defined: *)
+   the conclusion of the subroutine.  The "trueif_inv" function asserts that
+   anywhere an invariant exists (e.g., at the post-condition), it is true. *)
 Theorem strlen_preserves_esp:
-  forall s esp mem d n s' x
+  forall s esp mem d n s' x'
          (ESP0: s R_ESP = Ⓓ esp) (MEM0: s V_MEM32 = Ⓜ mem)
          (RET: strlen_i386 (mem Ⓓ[esp]) = None)
-         (XP0: exec_prog fh strlen_i386 0 s d n s' x),
-  match strlen_esp_inv mem esp x s' n with Some P => P | None => True end.
+         (XP0: exec_prog fh strlen_i386 0 s d n s' x'),
+  trueif_inv (strlen_esp_invset esp strlen_i386 x' s').
 Proof.
   intros.
 
-  (* First, simplify x to (Exit _) by observing that our invariant-set does not impose
-     any proof obligation when x is a non-standard exit condition (e.g., exception). *)
-  destruct x as [|a'|i]; try exact I.
-
-  (* Now use the prog_inv inductive principle from Picinae_theory.v. *)
-  eapply prog_inv. exact XP0.
+  (* Use the prove_inv inductive principle from Picinae_theory.v. *)
+  eapply prove_invs. exact XP0.
 
   (* We must first prove the pre-condition, which says that the invariant-set is
      satisfied on entry to the subroutine.  This is proved by assumption ESP0. *)
-  unfold strlen_esp_inv, x86_subroutine_inv. destruct (N.eq_dec _ _).
-    rewrite <- e in RET. discriminate RET.
-    exact ESP0.
+  exact ESP0.
 
   (* Now we enter the inductive case, wherein Coq asks us to prove that the invariant-set
      is preserved by every (reachable) instruction in the program.  Before breaking the
      goal down into many cases (one for each instruction in this case), it is wise to
-     simplify and/or remove anything in the context that is unnecessary.  We first
-     simplify the pre-condition assumption. *)
+     simplify and/or remove anything in the context that is unnecessary. In order for
+     symbolic interpretation to succeed, the context must reveal the values of all
+     relevant variables in store s1 (which denotes the store on entry to each instruction
+     for which the goal must be proved).  The only two variables in our invariant-set are
+     ESP and MEM.  The value of ESP will be revealed by our pre-condition (PRE).  We can
+     get the value of MEM from MEM0 using our previously proved strlen_preserves_memory
+     theorem. *)
   intros.
-  unfold strlen_esp_inv, x86_subroutine_inv in PRE. destruct (N.eq_dec a1 _).
-    subst a1. eapply NISStep. intros. rewrite IL in RET. discriminate RET.
-  unfold strlen_esp_invset in PRE.
-
-  (* In order for symbolic interpretation to succeed, the context must reveal the values
-     of all relevant variables in store s1 (which denotes the store on entry to each
-     instruction for which the goal must be proved).  The only two variables in our
-     invariant-set are ESP and MEM.  The value of ESP is already revealed by our
-     pre-condition (PRE).  We can get the value of MEM from MEM0 using our previously
-     proved strlen_preserves_memory theorem. *)
-  assert (MEM: s1 V_MEM32 = Some (VaM mem 32)).
+  assert (MEM: s1 V_MEM32 = Ⓜ mem).
     rewrite <- MEM0. eapply strlen_preserves_memory. exact XP.
-  clear n0 MEM0 XP0 XP.
+  clear s MEM0 XP0 ESP0 XP.
 
   (* We are now ready to break the goal down into one case for each invariant-point.
-     The destN tactic (defined above) recursively destructs address a1 into all
-     possible addresses.  To use it, you need to give it a tactic-sequence that
-     eliminates the goal whenever a1 is not the address of any instruction.  Usually
-     the best way to do that is to temporarily set a1 to a non-instruction address
-     (e.g., replace a1 with 1) and then figure out how to disprove the resulting goal
-     by contradiction.  In this case, discrimination on IL works.  Once you have a
-     tactic sequence that disproves non-instruction goals, use it as the "until"
-     argument to destN: *)
-  destN a1 until (apply NISStep; intros; discriminate IL) eqn:ADDR.
+     The shelve_cases tactic finds all the invariants defined by the invariant-set
+     in a precondition hypothesis (PRE).  Its first argument is the address bitwidth
+     of the ISA (32 bits in this case).  After shelve_cases, use Coq's "Unshelve"
+     command to recover the list of goals that the tactic "shelved" for you. *)
+  shelve_cases 32 PRE.
+  Unshelve.
 
-  (* We now have one goal for each invariant-point.  We must prove that each of these
-     instructions preserves the invariant-set.  To do so, we apply the symbolic
-     interpreter to all the goals in parallel.  (Note that this can take a while.)
-     If this fails, you should do "try x86_step" instead, and then try to figure out
-     why some steps didn't work.  It's usually because you forgot to derive the
-     value of some IL variable needed by the symbolic interpreter to make progress
-     on that subgoal. *)
+  (* Now we launch the symbolic interpreter on all goals in parallel.  (This can
+     take a while to complete, so please be patient...!) *)
   all: x86_step.
 
   (* Note that we wind up with more goals that we started with, since some of the
@@ -198,25 +140,75 @@ Proof.
      Fortunately, since this is a pretty simple invariant-set, the symbolic state
      inferred for most of the goals trivially satisfies the theorem.  We can solve
      all but one by assumption or reflexivity: *)
-  all: try solve [ exact PRE | reflexivity ].
+  all: try solve [ reflexivity | assumption ].
 
   (* The only unsolved goal is the one for the final instruction in the program,
      which is the only one that modifies ESP.  We can solve that one using the
      update_updated theorem, which reasons about state updates. *)
-  unfold strlen_esp_postcond.
   apply update_updated.
+
+  (* At Qed, Coq re-checks the proof, including all those symbolic interpretation
+     steps, so please be patient again... *)
 Qed.
 
 
 
+
 (* Example #4: Partial correctness
-   At termination, strlen returns (in EAX) a value k that satisfies the following:
+   Proving full partial correctness of strlen is challenging because strlen's
+   binary implementation relies on some obscure properties of bit arithmetic
+   to more efficiently find zeros in groups of bytes instead of one at a time.
+   Our goal is to prove that at termination, strlen returns (in EAX) a value k
+   that satisfies the following:
    (1) p <= k,
    (2) no memory byte at addresses in the interval [p, p+k) is nil, and
    (3) the byte at address p+k is nil,
    where p is the address stored at [ESP+4] on entry. *)
 
+(* We define partial-correctness of strlen as returning an index in EAX
+   such that all addresses in [p, p+EAX) are "nil-free" (non-zero), where
+   p is the (original) value of the first stack argument. *)
+Definition nilfree (m:addr->N) (p:addr) (k:N) :=
+  p <= k /\ forall i, p <= i -> i < k -> m i > 0.
+
+(* The invariant-set for this property is much more complex than our previous
+   examples.  At the entrypoint (address 0) we have no assumptions (True).
+   Addresses 38, 153, and 182 are meets in the control-flow graph, so we place
+   invariants at those points to simplify the analysis.  Address 49 is the
+   start of an unrolled loop, where the loop body has been replicated at
+   addresses 75, 101, and 127 for better performance.  We therefore put our
+   loop invariant at all four addresses so that we can treat it like a rolled
+   loop, and avoid duplications in the proof logic.  Address 186 is the
+   return instruction at the end, so gets a special invariant. *)
 Definition ones (b n:N) := N.iter n (fun x => x * 2^b + 1) 0.
+Definition strlen_invs (m:addr->N) (esp:N) (a:addr) (s:store) :=
+  match a with
+  | 0 => Some True
+  | 38 => Some (∃ eax edx, s R_EAX = Ⓓeax /\ s R_EDX = Ⓓedx /\ nilfree m (m Ⓓ[esp+4]) eax /\ edx < 4)
+  | 49 | 75 | 101 | 127 => Some (∃ eax, s R_EAX = Ⓓeax /\ nilfree m (m Ⓓ[esp+4]) eax /\ s R_EDX = Ⓓ0)
+  | 153 => Some (∃ eax, s R_EAX = Ⓓeax /\ nilfree m (m Ⓓ[esp+4]) (eax-4) /\ 4 <= eax /\
+                         s R_ECX = Ⓓ(2^32 + m Ⓓ[eax-4] ⊖ ones 8 4) /\
+                         exists i, m Ⓓ[esp+4] <= i < eax /\ m i = 0)
+  | 182 => Some (∃ eax, s R_EAX = Ⓓeax /\ nilfree m (m Ⓓ[esp+4]) eax /\ m eax = 0)
+  | 186 => Some (∃ eax, s R_EAX = Ⓓeax /\ nilfree m (m Ⓓ[esp+4]) ((m Ⓓ[esp+4])+eax) /\ m ((m Ⓓ[esp+4])+eax) = 0)
+  | _ => None
+  end.
+
+(* The post-condition says that ESP gets restored and EAX is the index of the
+   first nil character after input pointer p. *)
+Definition strlen_post (mem:addr->N) (esp:N) (_:exit) (s:store) :=
+  s R_ESP = Ⓓ (esp+4) /\
+  let p := mem Ⓓ[esp+4] in
+  exists eax, s R_EAX = Ⓓ eax /\
+              mem (p + eax) = 0 /\
+              forall i, i < eax -> mem (p+i) > 0.
+
+(* The invariant-set and post-conditions are combined as usual: *)
+Definition strlen_invset (mem:addr->N) (esp:N) :=
+  invs (strlen_invs mem esp) (strlen_post mem esp).
+
+(* Before attempting the main theorem, we prove a large collection of helper lemmas
+   about bit arithmetic... *)
 
 Lemma land_lohi_0:
   forall x y n, x < 2^n -> N.land x (N.shiftl y n) = 0.
@@ -718,56 +710,14 @@ Proof.
     exact MK.
 Qed.
 
-
-(* We define partial-correctness of strlen as returning an index in EAX
-   such that all addresses in [p, p+EAX) are "nil-free" (non-zero), where
-   p is the (original) value of the first stack argument. *)
-Definition nilfree (m:addr->N) (p:addr) (k:N) :=
-  p <= k /\ forall i, p <= i -> i < k -> m i > 0.
-
-(* The invariant-set for this property is much more complex than our previous
-   examples.  At the entrypoint (address 0) we have no assumptions (True).
-   Addresses 38, 153, and 182 are meets in the control-flow graph, so we place
-   invariants at those points to simplify the analysis.  Address 49 is the
-   start of an unrolled loop, where the loop body has been replicated at
-   addresses 75, 101, and 127 for better performance.  We therefore put our
-   loop invariant at all four addresses so that we can treat it like a rolled
-   loop, and avoid duplications in the proof logic.  Address 186 is the
-   return instruction at the end, so gets a special invariant. *)
-Definition strlen_invset (m:addr->N) (esp:N) (a:addr) (_:exit) (s:store) (_:nat) :=
-  match a with
-  | 0 => Some True
-  | 38 => Some (∃ eax edx, s R_EAX = Ⓓeax /\ s R_EDX = Ⓓedx /\ nilfree m (m Ⓓ[esp+4]) eax /\ edx < 4)
-  | 49 | 75 | 101 | 127 => Some (∃ eax, s R_EAX = Ⓓeax /\ nilfree m (m Ⓓ[esp+4]) eax /\ s R_EDX = Ⓓ0)
-  | 153 => Some (∃ eax, s R_EAX = Ⓓeax /\ nilfree m (m Ⓓ[esp+4]) (eax-4) /\ 4 <= eax /\
-                         s R_ECX = Ⓓ(2^32 + m Ⓓ[eax-4] ⊖ ones 8 4) /\
-                         exists i, m Ⓓ[esp+4] <= i < eax /\ m i = 0)
-  | 182 => Some (∃ eax, s R_EAX = Ⓓeax /\ nilfree m (m Ⓓ[esp+4]) eax /\ m eax = 0)
-  | 186 => Some (∃ eax, s R_EAX = Ⓓeax /\ nilfree m (m Ⓓ[esp+4]) ((m Ⓓ[esp+4])+eax) /\ m ((m Ⓓ[esp+4])+eax) = 0)
-  | _ => None
-  end.
-
-(* The post-condition says that ESP gets restored and EAX is the index of the
-   first nil character after input pointer p. *)
-Definition strlen_postcond (mem:addr->N) (esp:N) (_:addr) (_:exit) (s:store) (_:nat) :=
-  s R_ESP = Ⓓ (esp+4) /\
-  let p := mem Ⓓ[esp+4] in
-  exists eax, s R_EAX = Ⓓ eax /\
-              mem (p + eax) = 0 /\
-              forall i, i < eax -> mem (p+i) > 0.
-
-(* The invariant-set and post-conditions are combined as usual: *)
-Definition strlen_inv (mem:addr->N) (esp:N) :=
-  x86_subroutine_inv strlen_i386 (strlen_invset mem esp) (strlen_postcond mem esp) (mem Ⓓ[esp]).
-
-(* Our premises for this theorem are a bit more elaborate.  Here is some rationale:
+(* Finally we're ready to prove the main partial correctness theorem.  Our premises
+   are a bit more elaborate than for previous examples.  Here is some rationale:
    (HI0) The theorem is only true if the search for a nil does not wrap
      around the address space and become lower than p.  In user code
      this can never happen because the high bytes of the address space
      are reserved and unreadable.  We therefore assume that the highest
      byte is unreadable.
-   (MDL0) Since we will be doing full symbolic interpretation, we must
-     assume that on entry the processor is in a valid state.
+   (MDL0) Assume that on entry the processor is in a valid state.
    (ESPLO) Also, the input stack pointer must not be beyond user memory,
      since otherwise "restoring" it would incur an integer overflow. *)
 Theorem strlen_partial_correctness:
@@ -778,20 +728,13 @@ Theorem strlen_partial_correctness:
          (ESP0: s R_ESP = Ⓓ esp) (MEM0: s V_MEM32 = Ⓜ mem)
          (RET: strlen_i386 (mem Ⓓ[esp]) = None)
          (XP0: exec_prog fh strlen_i386 0 s d n s' x),
-  match strlen_inv mem esp x s' n with Some P => P | None => True end.
+  trueif_inv (strlen_invset mem esp strlen_i386 x s').
 Proof.
   intros.
-
-  (* Our invariant is trivially satisfied by non-standard exit conditions. *)
-  destruct x as [|a'|i]; try exact I.
-
-  (* Use the prog_inv inductive principle. *)
-  eapply prog_inv. exact XP0.
+  eapply prove_invs. exact XP0.
 
   (* The pre-condition (True) is trivially satisfied. *)
-  unfold strlen_inv, x86_subroutine_inv. destruct (N.eq_dec _ _).
-    rewrite <- e in RET. discriminate RET.
-    exact I.
+  exact I.
 
   (* Before splitting into cases, translate each hypothesis about the
      entry point store s to each instruction's starting store s1: *)
@@ -808,20 +751,14 @@ Proof.
   assert (ESP := strlen_preserves_esp _ _ _ _ _ _ (Exit a1) ESP0 MEM0 RET XP).
   clear s HI0 MDL0 MEM0 ESP0 XP XP0.
 
-  (* Eliminate the case where address a1 does not contain an instruction. *)
-  unfold strlen_inv, strlen_esp_inv, x86_subroutine_inv in PRE, ESP.
-  destruct (N.eq_dec a1 _). subst a1. eapply NISStep. intros. rewrite IL in RET. discriminate RET.
-  clear n0.
-
   (* Break the proof into cases, one for each invariant-point. *)
-  destN a1 until (exfalso; exact PRE) eqn:ADDR.
-  all: unfold strlen_invset in PRE; unfold strlen_esp_invset in ESP.
+  shelve_cases 32 PRE. Unshelve.
 
   (* Time how long it takes for each symbolic interpretation step to complete
      (for profiling and to give visual cues that something is happening...). *)
   Local Ltac step := time x86_step.
 
-  all: focus_addr ADDR 0. clear PRE.
+  (* Address 0 *)
   step. rewrite N.mod_small by (eapply N.lt_le_trans; [|exact ESPLO]; apply N.add_lt_mono_l; reflexivity).
   step.
   step.
@@ -863,7 +800,7 @@ Proof.
   eexists. eexists. do 2 (split; [reflexivity|]). split. exact NF2. apply N.mod_upper_bound. discriminate 1.
   eexists. eexists. do 2 (split; [reflexivity|]). split. exact NF0. apply N.mod_upper_bound. discriminate 1.
 
-  Unshelve. all: focus_addr ADDR 38. destruct PRE as [eax [edx [EAX [EDX [NF EDX4]]]]].
+  (* Address 38 *) destruct PRE as [eax [edx [EAX [EDX [NF EDX4]]]]].
   step. assert (LM3: eax + 1 < 2^32).
     apply N.lt_nge. intro H. apply HI.
     replace eax with (2^32-1) in ACC. apply (ACC 0). reflexivity.
@@ -878,17 +815,17 @@ Proof.
       revert i H1 H2. exact (proj2 NF).
       rewrite H2. apply N_neq0_gt0, N.neq_sym, N.eqb_neq, BC.
 
-  Unshelve. all: match type of ADDR with _=49 => idtac | _=75 => idtac | _=101 => idtac | _=127 => idtac | _ => shelve end.
-  all: unfold strlen_invset in PRE; destruct PRE as [eax [EAX [NF EDX0]]].
-  all:step. all:assert (LM: eax + 4 < 2^32) by (apply N.lt_nge; intro H; apply HI;
+  (* Addresses 49, 75, 101, 127 *)
+  1-4: unfold strlen_invset in PRE; destruct PRE as [eax [EAX [NF EDX0]]].
+  1-4:step. 1-4:assert (LM: eax + 4 < 2^32) by (apply N.lt_nge; intro H; apply HI;
     replace (2^32-1) with (eax+(N.pred(2^32) - eax));
     [ apply ACC, (N.add_lt_mono_r _ _ eax); rewrite N.sub_add by apply N.lt_le_pred, (x86_regsize MDL EAX); rewrite N.add_comm; eapply N.lt_le_trans; [|exact H]; reflexivity
     | rewrite N.add_sub_assoc by apply N.lt_le_pred, (x86_regsize MDL EAX); rewrite N.add_comm, N.add_sub; reflexivity ]).
-  all:step.
-  all:step.
-  all:step. all:change 4278124287 with (2^32 - ones 8 4).
-  all:step.
-  all:step.
+  1-4:step.
+  1-4:step.
+  1-4:step. 1-4:change 4278124287 with (2^32 - ones 8 4).
+  1-4:step.
+  1-4:step.
   2,4,6,8:apply N.ltb_ge, le_add_sub_mod in BC; [|reflexivity];
   eexists; split; [reflexivity|]; rewrite N.add_sub; split; [exact NF|]; repeat split;
   [ rewrite N.add_comm; apply N.le_add_r
@@ -897,17 +834,17 @@ Proof.
     [ etransitivity; [ apply (proj1 NF) | apply N.le_add_r ]
     | apply N.add_lt_mono_l; exact I4
     | exact NIL ] ].
-  all: apply N.ltb_lt, add_sub_mod_le in BC; [|discriminate 1].
-  all: rewrite sub_lnot by apply getmem_bound, WTM.
-  all:step.
-    all:rewrite N.add_sub_assoc by discriminate 1.
-    all:rewrite (N.add_comm _ (2^32)).
-    all:rewrite <- N.add_sub_assoc by exact BC.
-    all:rewrite N.add_mod, N.mod_same, N.add_0_l, N.mod_mod by (apply N.pow_nonzero; discriminate 1).
-    all:rewrite (N.mod_small (_-_)) by (eapply N.le_lt_trans; [ apply N.le_sub_l | apply getmem_bound, WTM ]).
-  all:change 16843008 with (ones 8 4 - 1).
-  all:step.
-  all:step.
+  1-4: apply N.ltb_lt, add_sub_mod_le in BC; [|discriminate 1].
+  1-4: rewrite sub_lnot by apply getmem_bound, WTM.
+  1-4:step.
+    1-4:rewrite N.add_sub_assoc by discriminate 1.
+    1-4:rewrite (N.add_comm _ (2^32)).
+    1-4:rewrite <- N.add_sub_assoc by exact BC.
+    1-4:rewrite N.add_mod, N.mod_same, N.add_0_l, N.mod_mod by (apply N.pow_nonzero; discriminate 1).
+    1-4:rewrite (N.mod_small (_-_)) by (eapply N.le_lt_trans; [ apply N.le_sub_l | apply getmem_bound, WTM ]).
+  1-4:change 16843008 with (ones 8 4 - 1).
+  1-4:step.
+  1-4:step.
   1,3,5,7:apply Neqb_ok in BC0; symmetry in BC0; eexists; split; [reflexivity|]; repeat split;
   [ etransitivity; [ apply (proj1 NF) | apply N.le_add_r ]
   | intros; destruct (N.lt_ge_cases i eax);
@@ -916,7 +853,7 @@ Proof.
       (apply noborrow_nonil with (w:=4); try assumption);
       apply (N.add_lt_mono_l _ _ eax); rewrite N.add_sub_assoc, N.add_comm, N.add_sub; assumption ]
   | rewrite BC0; reflexivity ].
-  all: eexists; split; [reflexivity|]; rewrite N.add_sub; split; [exact NF|]; repeat split;
+  1-4: eexists; split; [reflexivity|]; rewrite N.add_sub; split; [exact NF|]; repeat split;
   [ rewrite N.add_comm; apply N.le_add_r
   | rewrite <- N.add_sub_assoc by exact BC; rewrite <- N.add_mod_idemp_l, N.mod_same, N.add_0_l by discriminate 1;
     rewrite N.mod_small; [reflexivity|]; eapply N.le_lt_trans; [apply N.le_sub_l | apply getmem_bound,WTM ]
@@ -926,7 +863,7 @@ Proof.
     | apply N.add_lt_mono_l, I4
     | exact NIL ] ].
 
-  Unshelve. all:focus_addr ADDR 153. destruct PRE as [eax [EAX [NF [EAX4 [ECX NIL]]]]].
+  (* Address 153 *) destruct PRE as [eax [EAX [NF [EAX4 [ECX NIL]]]]].
   step.
     rewrite <- N.add_sub_assoc by exact EAX4.
     rewrite <- N.add_mod_idemp_l, N.mod_same, N.add_0_l by discriminate 1.
@@ -1009,7 +946,7 @@ Proof.
       rewrite <- H2. exact NIL.
     rewrite N.sub_1_r. apply N.succ_pred. intro H. apply EAX4. rewrite H. reflexivity.
 
-  Unshelve. all:focus_addr ADDR 182. destruct PRE as [eax [EAX [NF NIL]]].
+  (* Address 182 *) destruct PRE as [eax [EAX [NF NIL]]].
   step.
     rewrite (N.mod_small (esp+4)) by (eapply N.lt_le_trans; [|exact ESPLO]; apply N.add_lt_mono_l; reflexivity).
     rewrite <- N.add_sub_assoc by exact (proj1 NF).
@@ -1019,7 +956,7 @@ Proof.
     exact NF.
     exact NIL.
 
-  Unshelve. destruct PRE as [eax [EAX [NF NIL]]].
+  (* Address 186 *) destruct PRE as [eax [EAX [NF NIL]]].
   step. split. simpl_stores. rewrite N.mod_small. reflexivity. eapply N.lt_le_trans; [|exact ESPLO]. apply N.add_lt_mono_l. reflexivity.
   eexists. simpl_stores. repeat split.
     exact EAX.
